src/Init/Data/Float.lean
@@ -265,11 +265,17 @@ instance : ToString Float where
   toString := Float.toString
 
 /-- Obtains the `Float` whose value is the same as the given `UInt8`. -/
-@[extern "lean_uint8_to_float"] opaque UInt8.toFloat (n : UInt8) : Float
+@[extern "lean_uint8_to_float"] def UInt8.toFloat (n : UInt8) : Float :=
+  ⟨.ofNat n.toNat⟩
+
 /-- Obtains the `Float` whose value is the same as the given `UInt16`. -/
-@[extern "lean_uint16_to_float"] opaque UInt16.toFloat (n : UInt16) : Float
+@[extern "lean_uint16_to_float"] def UInt16.toFloat (n : UInt16) : Float :=
+  ⟨.ofNat n.toNat⟩
+
 /-- Obtains the `Float` whose value is the same as the given `UInt32`. -/
-@[extern "lean_uint32_to_float"] opaque UInt32.toFloat (n : UInt32) : Float
+@[extern "lean_uint32_to_float"] def UInt32.toFloat (n : UInt32) : Float :=
+  ⟨.ofNat n.toNat⟩
+
 /--
 Obtains a `Float` whose value is near the given `UInt64`.
 
@@ -277,10 +283,11 @@ It will be exactly the value of the given `UInt64` if such a `Float` exists. If 
 exists, the returned value will either be the smallest `Float` that is larger than the given value,
 or the largest `Float` that is smaller than the given value.
 
-This function is opaque in the kernel, but is overridden at runtime with an efficient
-implementation.
+This function is overridden at runtime with an efficient implementation.
 -/
-@[extern "lean_uint64_to_float"] opaque UInt64.toFloat (n : UInt64) : Float
+@[extern "lean_uint64_to_float"] def UInt64.toFloat (n : UInt64) : Float :=
+  ⟨.ofNat n.toNat⟩
+
 /--
 Obtains a `Float` whose value is near the given `USize`.
 
@@ -288,10 +295,10 @@ It will be exactly the value of the given `USize` if such a `Float` exists. If n
 exists, the returned value will either be the smallest `Float` that is larger than the given value,
 or the largest `Float` that is smaller than the given value.
 
-This function is opaque in the kernel, but is overridden at runtime with an efficient
-implementation.
+This function is overridden at runtime with an efficient implementation.
 -/
-@[extern "lean_usize_to_float"] opaque USize.toFloat (n : USize) : Float
+@[extern "lean_usize_to_float"] def USize.toFloat (n : USize) : Float :=
+  ⟨.ofNat n.toNat⟩
 
 instance : Inhabited Float where
   default := UInt64.toFloat 0
