src/Init/Data/SInt/Float32.lean
@@ -68,45 +68,40 @@ This function does not reduce in the kernel.
 -/
 @[extern "lean_float32_to_isize"] opaque Float32.toISize : Float32 → ISize
 
-/--
-Obtains the `Float32` whose value is the same as the given `Int8`.
+/-- Obtains the `Float32` whose value is the same as the given `Int8`. -/
+@[extern "lean_int8_to_float32"] def Int8.toFloat32 (n : Int8) : Float32 :=
+  ⟨.ofInt n.toInt⟩
 
-This function does not reduce in the kernel.
--/
-@[extern "lean_int8_to_float32"] opaque Int8.toFloat32 (n : Int8) : Float32
-/--
-Obtains the `Float32` whose value is the same as the given `Int16`.
+/-- Obtains the `Float32` whose value is the same as the given `Int16`. -/
+@[extern "lean_int16_to_float32"] def Int16.toFloat32 (n : Int16) : Float32 :=
+  ⟨.ofInt n.toInt⟩
 
-This function does not reduce in the kernel.
--/
-@[extern "lean_int16_to_float32"] opaque Int16.toFloat32 (n : Int16) : Float32
 /--
 Obtains a `Float32` whose value is near the given `Int32`.
 
 It will be exactly the value of the given `Int32` if such a `Float32` exists. If no such `Float32`
 exists, the returned value will either be the smallest `Float32` that is larger than the given
 value, or the largest `Float32` that is smaller than the given value.
-
-This function does not reduce in the kernel.
 -/
-@[extern "lean_int32_to_float32"] opaque Int32.toFloat32 (n : Int32) : Float32
+@[extern "lean_int32_to_float32"] def Int32.toFloat32 (n : Int32) : Float32 :=
+  ⟨.ofInt n.toInt⟩
+
 /--
 Obtains a `Float32` whose value is near the given `Int64`.
 
 It will be exactly the value of the given `Int64` if such a `Float32` exists. If no such `Float32`
 exists, the returned value will either be the smallest `Float32` that is larger than the given
 value, or the largest `Float32` that is smaller than the given value.
-
-This function does not reduce in the kernel.
 -/
-@[extern "lean_int64_to_float32"] opaque Int64.toFloat32 (n : Int64) : Float32
+@[extern "lean_int64_to_float32"] def Int64.toFloat32 (n : Int64) : Float32 :=
+  ⟨.ofInt n.toInt⟩
+
 /--
 Obtains a `Float32` whose value is near the given `ISize`.
 
 It will be exactly the value of the given `ISize` if such a `Float32` exists. If no such `Float32`
 exists, the returned value will either be the smallest `Float32` that is larger than the given
 value, or the largest `Float32` that is smaller than the given value.
-
-This function does not reduce in the kernel.
 -/
-@[extern "lean_isize_to_float32"] opaque ISize.toFloat32 (n : ISize) : Float32
+@[extern "lean_isize_to_float32"] def ISize.toFloat32 (n : ISize) : Float32 :=
+  ⟨.ofInt n.toInt⟩
